theories/logrel/rel_rules.v
@@ -4,7 +4,7 @@ From stdpp Require Import coPset namespaces.
 From iris.proofmode Require Import proofmode.
 From iris.algebra Require Import list.
 From self.program_logic Require Import ectx_lifting.
-From self.prob_lang Require Import lang spec_rules spec_tactics ctx_subst proofmode.
+From self.prob_lang Require Import lang spec_rules spec_tactics proofmode.
 From self.logrel Require Import model.
 
 Section rules.
@@ -21,60 +21,49 @@ Section rules.
 
   (** ** Forward reductions on the LHS *)
 
-  Lemma refines_pure_l n
+  Lemma refines_pure_l E n
     (K' : list ectx_item) e e' t A ϕ :
     PureExec ϕ n e e' →
     ϕ →
-    ▷^n (REL fill K' e' << t : A)
-    ⊢ REL fill K' e << t : A.
-  Proof.
-    intros Hpure Hϕ.
-    rewrite refines_eq /refines_def.
-    iIntros "IH" (j) "Hs Hnais".
-    iModIntro. wp_pures.
-    iApply fupd_wp. iApply ("IH" with "Hs Hnais").
-  Qed.
-
-  Lemma refines_masked_l E n
-    (K' : list ectx_item) e e' t A ϕ :
-    PureExec ϕ n e e' →
-    ϕ →
-    (REL fill K' e' << t @ E : A)
+    ▷^n (REL fill K' e' << t @ E : A)
     ⊢ REL fill K' e << t @ E : A.
   Proof.
     intros Hpure Hϕ.
     rewrite refines_eq /refines_def.
-    iIntros "IH" (j) "Hs Hnais /=".
-    iMod ("IH" with "Hs Hnais") as "IH".
-    iModIntro. by wp_pures.
+    iIntros "IH" (j) "Hs Hnais".
+    wp_pures.
+    iApply ("IH" with "Hs Hnais").
   Qed.
 
-  Lemma refines_wp_l K e1 t A :
-    (WP e1 {{ v,
-        REL fill K (of_val v) << t : A }})%I -∗
-    REL fill K e1 << t : A.
+  Lemma refines_wp_l E K e1 t A :
+    (WP e1 @ E {{ v,
+        REL fill K (of_val v) << t @ E : A }})%I -∗
+    REL fill K e1 << t @ E : A.
   Proof.
     rewrite refines_eq /refines_def.
-    iIntros "He" (j) "Hs Hnais /=".
-    iModIntro. iApply wp_bind.
+    iIntros "He" (K') "Hs Hnais /=".
+    iApply wp_bind.
     iApply (wp_wand with "He").
     iIntros (v) "Hv".
-    by iMod ("Hv" with "Hs Hnais").
+    iApply ("Hv" with "Hs Hnais").
   Qed.
 
-  Lemma refines_atomic_l (E : coPset) K e1 t A
-        (Hatomic : Atomic WeaklyAtomic e1) :
-   (|={⊤,E}=> WP e1 @ E {{ v,
-     REL fill K (of_val v) << t @ E : A }})%I -∗
-   REL fill K e1 << t : A.
+  Lemma refines_atomic_l (E1 E2 : coPset) K e1 t A
+    (Hatomic : Atomic WeaklyAtomic e1) :
+    (∀ K', refines_right K' t ={E1,E2}=∗
+             WP e1 @ E2 {{ v,
+              |={E2, E1}=> ∃ t', refines_right K' t' ∗
+              REL fill K (of_val v) << t' @ E1 : A }})%I -∗
+   REL fill K e1 << t @ E1 : A.
   Proof.
     rewrite refines_eq /refines_def.
-    iIntros "Hlog" (j) "Hs Hnais /=". iModIntro.
+    iIntros "Hlog" (K') "Hs Hnais /=".
     iApply wp_bind. iApply wp_atomic; auto.
-    iMod "Hlog" as "He". iModIntro.
+    iMod ("Hlog" with "Hs") as "He". iModIntro.
     iApply (wp_wand with "He").
     iIntros (v) "Hlog".
-    by iApply ("Hlog" with "Hs Hnais").
+    iMod "Hlog" as (t') "[Hr Hlog]".
+    iApply ("Hlog" with "Hr Hnais").
   Qed.
 
   (** ** Forward reductions on the RHS *)
@@ -181,10 +170,10 @@ Section rules.
   Qed.
 
   (** This rule is useful for proving that functions refine each other *)
-  Lemma refines_arrow_val (v v' : val) A A' :
+  Lemma refines_arrow_val E1 E2 (v v' : val) A A' :
     □(∀ v1 v2, A v1 v2 -∗
-      REL App v (of_val v1) << App v' (of_val v2) : A') -∗
-    REL (of_val v) << (of_val v') : (A → A')%lrel.
+      REL App v (of_val v1) << App v' (of_val v2) @ E2 : A') -∗
+    REL (of_val v) << (of_val v') @ E1 : (A →{E2} A')%lrel.
   Proof.
     iIntros "#H".
     iApply refines_ret. iModIntro.
@@ -199,66 +188,60 @@ Section rules.
 
   Lemma refines_alloc_l K E e v t A :
     IntoVal e v →
-    (|={⊤,E}=> ▷ (∀ l : loc, l ↦ v -∗
-           REL fill K (of_val #l) << t @ E : A))%I
-    -∗ REL fill K (ref e) << t : A.
+    (▷ (∀ l : loc, l ↦ v -∗
+           REL fill K (of_val #l) << t @ E : A))
+    -∗ REL fill K (ref e) << t @ E : A.
   Proof.
     iIntros (<-) "Hlog".
-    iApply refines_atomic_l; auto.
-    iMod "Hlog". iModIntro.
+    iApply refines_wp_l.
     wp_alloc l. by iApply "Hlog".
   Qed.
 
   Lemma refines_load_l K E l q t A :
-    (|={⊤,E}=> ∃ v',
+    (∃ v',
       ▷(l ↦{q} v') ∗
-      ▷(l ↦{q} v' -∗ (REL fill K (of_val v') << t @ E : A)))%I
-    -∗ REL fill K (! #l) << t : A.
+      ▷(l ↦{q} v' -∗ (REL fill K (of_val v') << t @ E : A)))
+    -∗ REL fill K (! #l) << t @ E : A.
   Proof.
-    iIntros "Hlog".
-    iApply refines_atomic_l; auto.
-    iMod "Hlog" as (v') "[Hl Hlog]". iModIntro.
+    iIntros "[%v' [Hl Hlog]]".
+    iApply refines_wp_l.
     wp_load. by iApply "Hlog".
   Qed.
 
   Lemma refines_store_l K E l e v' t A :
     IntoVal e v' →
-    (|={⊤,E}=> ∃ v, ▷ l ↦ v ∗
+    (∃ v, ▷ l ↦ v ∗
       ▷(l ↦ v' -∗ REL fill K (of_val #()) << t @ E : A))
-    -∗ REL fill K (#l <- e) << t : A.
+    -∗ REL fill K (#l <- e) << t @ E : A.
   Proof.
-    iIntros (<-) "Hlog".
-    iApply refines_atomic_l; auto.
-    iMod "Hlog" as (v) "[Hl Hlog]". iModIntro.
+    iIntros (<-) "[%v [Hl Hlog]]".
+    iApply refines_wp_l.
     wp_store. by iApply "Hlog".
   Qed.
 
   Lemma refines_alloctape_l K E t A :
-    (|={⊤,E}=> ▷ (∀ α : loc, α ↪ [] -∗
-           REL fill K (of_val #lbl:α) << t @ E : A))%I
-    -∗ REL fill K alloc << t : A.
+    (▷ (∀ α : loc, α ↪ [] -∗
+           REL fill K (of_val #lbl:α) << t @ E : A))
+    -∗ REL fill K alloc << t @ E : A.
   Proof.
     iIntros "Hlog".
-    iApply refines_atomic_l; auto.
-    iMod "Hlog". iModIntro.
-    iApply (wp_alloc_tape _ _ with "[//]"). iIntros "!>" (l) "?". by iApply "Hlog".
+    iApply refines_wp_l.
+    by wp_apply (wp_alloc_tape with "[//]").
   Qed.
 
-  Lemma refines_flip_l E K α b bs t A :
-    (|={⊤,E}=> ▷ α ↪ (b :: bs)
-               ∗ ▷ (α ↪ bs -∗ REL fill K (of_val #b) << t @ E : A))
-    -∗ REL fill K (flip #lbl:α) << t : A.
+  Lemma refines_flip_l E K α t A b bs :
+    (▷ α ↪ (b :: bs) ∗
+       ▷ (α ↪ bs -∗ REL fill K (of_val #b) << t @ E : A))
+    -∗ REL fill K (flip #lbl:α) << t @ E : A.
   Proof.
-    iIntros "Hlog".
-    iApply refines_atomic_l.
-    iMod "Hlog" as "[Hα Hlog]". iModIntro.
-    iApply (wp_flip with "Hα").
-    by iApply "Hlog".
+    iIntros "[Hα Hlog]".
+    iApply refines_wp_l.
+    by wp_apply (wp_flip with "Hα").
   Qed.
 
   Lemma refines_wand E e1 e2 A A' :
     (REL e1 << e2 @ E : A) -∗
-    (∀ v1 v2, A v1 v2 ={⊤}=∗ A' v1 v2) -∗
+    (∀ v1 v2, A v1 v2 ={E}=∗ A' v1 v2) -∗
     REL e1 << e2 @ E : A'.
   Proof.
     iIntros "He HAA".
@@ -267,10 +250,10 @@ Section rules.
     by iApply "HAA".
   Qed.
 
-  Lemma refines_arrow (v v' : val) A A' :
-    □ (∀ v1 v2 : val, □(REL of_val v1 << of_val v2 : A) -∗
-      REL App v (of_val v1) << App v' (of_val v2) : A') -∗
-    REL (of_val v) << (of_val v') : (A → A')%lrel.
+  Lemma refines_arrow E1 E2 (v v' : val) A A' :
+    □ (∀ v1 v2 : val, □(REL of_val v1 << of_val v2 @ E1 : A) -∗
+      REL App v (of_val v1) << App v' (of_val v2) @ E2 : A') -∗
+    REL (of_val v) << (of_val v') @ E1 : (A →{E2} A')%lrel.
   Proof.
     iIntros "#H".
     iApply refines_arrow_val; eauto.
@@ -279,77 +262,24 @@ Section rules.
     by iApply refines_ret.
   Qed.
 
-
-  Lemma refines_couple_tapes e1 e2 A α αₛ bs bsₛ :
+  Lemma refines_couple_tapes E e1 e2 A α αₛ bs bsₛ
+    (Hmasked : nclose specN ⊆ E) :
     to_val e1 = None →
     ((αₛ ↪ₛ bsₛ ∗ α ↪ bs ∗
        ((∃ b, αₛ ↪ₛ (bsₛ ++ [b]) ∗ α ↪ (bs ++ [b]))
-       -∗ REL e1 << e2 : A)))
-    ⊢ REL e1 << e2 : A.
+       -∗ REL e1 << e2 @ E : A)))
+    ⊢ REL e1 << e2 @ E : A.
   Proof.
     iIntros (e1ev) "(Hαs & Hα & Hlog)".
+    (* TODO: a separate [refines] lemma in [model] *)
     rewrite refines_eq /refines_def.
     iIntros (K2) "[#Hs He2] Hnais /=".
-    iApply wp_couple_tapes ; auto.
-    iSplitR ; auto.
-    iModIntro. rewrite -fupd_wp.
+    iApply wp_couple_tapes; [done|done|].
     iFrame "Hα Hαs".
-    iIntros "Hb".
-    iApply ("Hlog" with "Hb [Hs He2]") ; now iFrame.
-  Qed.
-
-  Lemma refines_couple_tapes_masked E e1 e2 A α αₛ bs bsₛ
-    (Hmasked : nclose specN ⊆ E) :
-    to_val e1 = None →
-    (|={⊤,E}=>
-       (αₛ ↪ₛ bsₛ ∗ α ↪ bs ∗
-       ((∃ b, αₛ ↪ₛ (bsₛ ++ [b]) ∗ α ↪ (bs ++ [b]))
-       -∗ REL e1 << e2 @ E : A)))
-    ⊢ REL e1 << e2 : A.
-  Proof.
-    iIntros (e1ev) "H".
-    rewrite refines_eq /refines_def.
-    iIntros (K2) "[#Hs He2] Hnais /= !>".
-    rewrite wp_unfold /wp_pre /= e1ev.
-    iIntros (???) "([Hh1 Ht1] & Hspec)".
-    iMod "H" as "(Hαs & Hα & H)".
-    iInv specN as (ρ' e0' σ0' n) ">(Hspec0 & %Hexec & Hauth & Hheap & Htapes)" "Hclose".
-    iDestruct (spec_interp_auth_frag_agree with "Hspec Hspec0") as %<-.
-    iDestruct (ghost_map_lookup with "Htapes Hαs") as %?.
-    iDestruct (ghost_map_lookup with "Ht1 Hα") as %?.
-    iApply fupd_mask_intro; [set_solver|]; iIntros "Hclose'".
-    (* Get up to speed with the spec resource (tracked in spec_ctx) *)
-    iApply exec_coupl_det_r; [done|].
-    (* Do a coupled [state_step] on both sides  *)
-    iApply (exec_coupl_state_steps α αₛ).
-    { rewrite /= /get_active.
-      apply elem_of_list_In, in_prod;
-        apply elem_of_list_In, elem_of_elements, elem_of_dom; eauto. }
-    iExists _.
-    iSplit.
-    { iPureIntro. eapply Rcoupl_pos_R, Rcoupl_state_step; by apply elem_of_dom. }
-    iIntros (σ2 σ2' ((? & ? & [b [= -> ->]]) & ? & ?)).
-    (* Update our resources *)
-    iMod (spec_interp_update (e0', (state_upd_tapes <[αₛ:=tapes σ0' !!! αₛ ++ [b]]> σ0'))
-           with "Hspec Hspec0") as "[Hspec Hspec0]".
-    iDestruct (ghost_map_lookup with "Ht1 Hα") as %?%lookup_total_correct.
-    iDestruct (ghost_map_lookup with "Htapes Hαs") as %?%lookup_total_correct.
-    simplify_map_eq.
-    iMod (ghost_map_update (tapes σ1 !!! α ++ [b]) with "Ht1 Hα") as "[Ht1 Hα]".
-    iMod (ghost_map_update (tapes σ0' !!! αₛ ++ [b]) with "Htapes Hαs") as "[Htapes Hαs]".
-    (* Close the [spec_ctx] invariant again, so the assumption can access all invariants  *)
-    iMod "Hclose'" as "_".
-    iMod ("Hclose" with "[Hauth Hheap Hspec0 Htapes]") as "_".
-    { iModIntro. rewrite /spec_inv.
-      iExists _, _, (state_upd_tapes _ _), 0. simpl.
-      iFrame. rewrite exec_O dret_1_1 //. }
-    (* Our [WP] assumption with the updated resources now suffices to prove the goal *)
-    iSpecialize ("H" with "[Hα Hαs] [$Hs $He2] Hnais").
-    { iExists _. iFrame. }
-    iMod "H".
-    rewrite !wp_unfold /wp_pre /= e1ev.
-    iMod ("H" $! (state_upd_tapes _ _) with "[$Hh1 $Hspec Ht1]") as "Hwp"; [done|].
-    iModIntro. done.
+    iSplit; [done|].
+    iIntros "[%b [Hαs Hα]]".
+    iApply ("Hlog" with "[Hα Hαs] [$Hs $He2] Hnais").
+    iExists _. iFrame.
   Qed.
 
 End rules.
